examples/logic/ltl/concrGBArepScript.sml
@@ -1,8 +1,8 @@
-open HolKernel Parse bossLib boolLib gfgTheory listTheory optionTheory pred_setTheory
+open HolKernel Parse bossLib boolLib gfgTheory listTheory optionTheory pred_setTheory rich_listTheory arithmeticTheory
 
 open sptreeTheory ltlTheory generalHelpersTheory concrRepTheory concrltl2waaTheory
 
-val _ = new_theory "concrGBARep"
+val _ = new_theory "concrGBArep"
 
 val _ = monadsyntax.temp_add_monadsyntax();
 val _ = overload_on("monad_bind",``OPTION_BIND``);
@@ -28,85 +28,213 @@ val gba_trans_concr_def = Define`
 
 val GBA_TRANS_LEMM1 = store_thm
   ("GBA_TRANS_LEMM1",
-   ``!x s. (ALL_DISTINCT s) ∧ MEM x (gba_trans_concr s)
+   ``!x s. MEM x (gba_trans_concr s)
         ==> ((!l. MEM l s
                  ==> (?cE. MEM cE l
                    ∧ (MEM_SUBSET cE.pos x.pos)
                    ∧ (MEM_SUBSET cE.neg x.neg)
                    ∧ (MEM_SUBSET cE.sucs x.sucs)
                      ))
-        ∧ (?f. (x = FOLDR
+          ∧ (?f. let s_with_ind = GENLIST (λn. (EL n s,n)) (LENGTH s)
+               in
+                let x1 =
+                   FOLDR
                     (λsF e.
                      <|pos := sF.pos ⧺ e.pos; neg := sF.neg ⧺ e.neg;
                        sucs := sF.sucs ⧺ e.sucs|>)
-                    (concrEdge [] [] []) (MAP f s))
-            ∧ (!q. MEM q s ==> MEM (f q) q)))``,
+                    (concrEdge [] [] []) (MAP f s_with_ind)
+               in (cE_equiv x x1)
+                ∧ (!q i. MEM (q,i) s_with_ind
+                       ==> MEM (f (q,i)) q))
+        ∧ (ALL_DISTINCT x.pos ∧ ALL_DISTINCT x.neg
+           ∧ ALL_DISTINCT x.sucs))``,
    Q.HO_MATCH_ABBREV_TAC
-    `!x s. AD s ∧ MEM x (gba_trans_concr s) ==> A x s ∧ B x s`
-   >> `!x s. AD s ∧ MEM x (gba_trans_concr s) ==> A x s ∧ (A x s ==> B x s)`
+    `!x s. MEM x (gba_trans_concr s) ==> A x s ∧ B x s`
+   >> `!x s. MEM x (gba_trans_concr s) ==> A x s ∧ (A x s ==> B x s)`
       suffices_by fs[]
-   >> qunabbrev_tac `A` >> qunabbrev_tac `B` >> qunabbrev_tac `AD`
+   >> qunabbrev_tac `A` >> qunabbrev_tac `B`
    >> Induct_on `s` >> fs[gba_trans_concr_def] >> rpt strip_tac
-   >- (fs[d_conj_concr_def,FOLDR_LEMM4] >> qexists_tac `e1` >> simp[]
-       >> metis_tac[MEM_SUBSET_APPEND]
+   >- (fs[cE_equiv_def,MEM_EQUAL_def,MEM_SUBSET_def])
+   >- (fs[cE_equiv_def,MEM_EQUAL_def,MEM_SUBSET_def]
+       >> fs[d_conj_concr_def,FOLDR_LEMM4] >> qexists_tac `e1` >> simp[]
+       >> metis_tac[MEM_SUBSET_APPEND,nub_set,MEM_SUBSET_SET_TO_LIST]
       )
-   >- (fs[d_conj_concr_def,FOLDR_LEMM4]
+   >- (fs[cE_equiv_def,MEM_EQUAL_def,MEM_SUBSET_def]
+       >> fs[d_conj_concr_def,FOLDR_LEMM4]
        >> `∃cE.
             MEM cE l ∧ MEM_SUBSET cE.pos e2.pos ∧
             MEM_SUBSET cE.neg e2.neg ∧ MEM_SUBSET cE.sucs e2.sucs`
           by metis_tac[]
-       >> metis_tac[MEM_SUBSET_APPEND,MEM_SUBSET_TRANS]
+       >> qexists_tac `cE`
+       >> metis_tac[MEM_SUBSET_APPEND,MEM_SUBSET_TRANS,nub_set,
+                    MEM_SUBSET_SET_TO_LIST]
       )
-   >- (fs[d_conj_concr_def,FOLDR_LEMM4]
+   >- (Cases_on `s= []` >> fs[]
+    >- (fs[d_conj_concr_def,FOLDR_CONS,MEM_MAP]
+        >> qexists_tac `
+             λ(q,i).
+               if (q,i) = (h,0) then e1 else ARB`
+        >> simp[] >> fs[d_conj_concr_def,FOLDR_CONS,MEM_MAP]
+        >> simp[cE_equiv_def,nub_set,MEM_EQUAL_SET]
+       )
+    >- (fs[d_conj_concr_def,FOLDR_LEMM4]
        >> first_x_assum (qspec_then `e2` mp_tac) >> simp[] >> strip_tac
+       >> qabbrev_tac `s_ind = (GENLIST (λn. (EL n s,n)) (LENGTH s))`
        >> `∃f.
-           e2 =
-            FOLDR
+           cE_equiv e2
+               (FOLDR
               (λsF e.
                  <|pos := sF.pos ⧺ e.pos; neg := sF.neg ⧺ e.neg;
                   sucs := sF.sucs ⧺ e.sucs|>) (concrEdge [] [] [])
-              (MAP f s)
-              ∧ (!q. MEM q s ==> MEM (f q) q)` by metis_tac[]
-       >> qexists_tac `λq. if q = h then e1 else f q` >> simp[]
-       >> `MAP (λq. if q = h then e1 else f q) s = MAP f s` by (
-            metis_tac[MAP_LEMM]
-        )
-       >> rw[FOLDR_CONCR_EDGE]
-      )
+              (MAP f s_ind))
+          ∧ (!q i. MEM (q,i) s_ind ==> MEM (f (q,i)) q)
+          ∧ ALL_DISTINCT e2.pos ∧ ALL_DISTINCT e2.neg
+          ∧ ALL_DISTINCT e2.sucs` by metis_tac[]
+       >> qexists_tac `
+             λ(q,i).
+              if i = 0
+              then e1
+              else f (q,i-1)` >> simp[]
+       >> fs[FOLDR_CONCR_EDGE] >> fs[nub_append] >> rpt strip_tac
+       >> fs[concrEdge_component_equality]
+       >- (qunabbrev_tac `s_ind` >> fs[]
+               >> fs[cE_equiv_def] >> rw[MEM_EQUAL_SET,LIST_TO_SET_FILTER]
+               >> (simp[SET_EQ_SUBSET,SUBSET_DEF]
+                   >> strip_tac >> fs[GENLIST]
+                   >- (rpt strip_tac
+                       >> Q.HO_MATCH_ABBREV_TAC
+                           `MEM k (FOLDR (λe pr. (g e) ⧺ pr) [] L)`
+                       >- (`MEM e1 L`
+                             suffices_by metis_tac[MEM_SUBSET_SET_TO_LIST,
+                                                   FOLDR_APPEND_LEMM,SUBSET_DEF]
+                           >> qunabbrev_tac `L` >> simp[MEM_MAP]
+                           >> qexists_tac `(h,0)` >> fs[EL,MEM_GENLIST]
+                           >> simp[LENGTH_NOT_NULL,NULL_EQ]
+                          )
+                       >- (`?e. MEM e L ∧ (MEM k (g e))`
+                             suffices_by metis_tac[FOLDR_LEMM6]
+                           >> qunabbrev_tac `L` >> simp[MEM_MAP] >> fs[]
+                           >> `MEM k
+                                (FOLDR (λe pr. g e ⧺ pr) []
+                                 (MAP f (GENLIST (λn. (EL n s,n)) (LENGTH s))))`
+                               by metis_tac[MEM_EQUAL_SET]
+                            >> fs[FOLDR_LEMM6] >> qexists_tac `a` >> strip_tac
+                            >- (fs[MEM_MAP] >> qexists_tac `(FST y,SND y+1)`
+                                >> simp[] >> fs[MEM_GENLIST]
+                                >> Cases_on `SUC n=LENGTH s` >> fs[]
+                                >> metis_tac[EL,TL,DECIDE ``n+1 = SUC n``]
+                               )
+                            >- fs[]
+                          )
+                      )
+                   >- (rpt strip_tac >> fs[FOLDR_LEMM6,MEM_MAP]
+                    >- (rw[] >> fs[] >> Cases_on `s = []` >> fs[]
+                        >> disj2_tac >> Q.HO_MATCH_ABBREV_TAC `MEM k (g e2)`
+                        >> `MEM k
+                             (FOLDR (λe pr. g e ⧺ pr) []
+                              (MAP f (GENLIST (λn. (EL n s,n)) (LENGTH s))))`
+                           suffices_by metis_tac[MEM_EQUAL_SET]
+                        >> simp[FOLDR_LEMM6,MEM_GENLIST,MEM_MAP]
+                        >> qexists_tac `f (EL (LENGTH s) (h::s),LENGTH s − 1)`
+                        >> simp[]
+                        >> qexists_tac `(EL (LENGTH s) (h::s),LENGTH s − 1)`
+                        >> fs[] >> `0 < LENGTH s` by (Cases_on `s` >> fs[])
+                        >> rw[]
+                        >> `?n. SUC n = LENGTH s`
+                           by (Cases_on `LENGTH s` >> simp[])
+                        >> `n = LENGTH s -1` by simp[] >> metis_tac[EL,TL]
+                       )
+                    >- (fs[MEM_GENLIST] >> rw[] >> fs[]
+                        >> Cases_on `n = 0` >> fs[] >> disj2_tac
+                        >> Q.HO_MATCH_ABBREV_TAC `MEM k (g e2)`
+                        >> `MEM k
+                             (FOLDR (λe pr. g e ⧺ pr) []
+                                (MAP f (GENLIST (λn. (EL n s,n)) (LENGTH s))))`
+                            suffices_by metis_tac[MEM_EQUAL_SET]
+                        >> simp[FOLDR_LEMM6,MEM_GENLIST,MEM_MAP]
+                        >> qexists_tac `f (EL n (h::s),n-1)`
+                        >> simp[]
+                        >> qexists_tac `(EL n (h::s),n − 1)`
+                        >> fs[] >> `0 < n` by fs[]
+                        >> `?p. SUC p = n`
+                              by (Cases_on `n` >> simp[])
+                        >> `p = n -1` by simp[] >> metis_tac[EL,TL]
+                       )
+                  )
+                  )
+              )
+       >> qunabbrev_tac `s_ind` >> fs[]
+       >> Cases_on `i=0` >> fs[MEM_GENLIST]
+       >> `?p. SUC p = i` by (Cases_on `i` >> simp[])
+       >> rw[]
+       )
+       )
+   >- (fs[d_conj_concr_def] >> fs[FOLDR_LEMM4] >> fs[all_distinct_nub])
+   >- (fs[d_conj_concr_def] >> fs[FOLDR_LEMM4] >> fs[all_distinct_nub])
+   >- (fs[d_conj_concr_def] >> fs[FOLDR_LEMM4] >> fs[all_distinct_nub])
   );
 
 val GBA_TRANS_LEMM2 = store_thm
   ("GBA_TRANS_LEMM2",
-   ``!s f. (!q. MEM q s ==> MEM (f q) q)
-  ==> MEM (FOLDR
+   ``!s f. (!q i. ((q = EL i s) ∧ i < LENGTH s)
+                      ==> MEM (f i) q)
+         ==> ?x. cE_equiv x
+            (FOLDR
                 (λsF e.
                      <|pos := sF.pos ⧺ e.pos; neg := sF.neg ⧺ e.neg;
                  sucs := sF.sucs ⧺ e.sucs|>)
-                (concrEdge [] [] []) (MAP f s)) (gba_trans_concr s)``,
+                (concrEdge [] [] []) (MAP f (COUNT_LIST (LENGTH s))))
+            ∧ MEM x(gba_trans_concr s)``,
    Induct_on `s` >> fs[gba_trans_concr_def]
-   >> rw[FOLDR_CONCR_EDGE] >> first_x_assum (qspec_then `f` mp_tac) >> simp[]
-   >> rpt strip_tac >> simp[d_conj_concr_def] >> rw[FOLDR_LEMM4]
-   >> qexists_tac `f h` >> fs[]
-   >> qexists_tac `(FOLDR
-                        (λsF e.
-                             <|pos := sF.pos ⧺ e.pos; neg := sF.neg ⧺ e.neg;
-                         sucs := sF.sucs ⧺ e.sucs|>) (concrEdge [] [] [])
-                        (MAP f s))`
-   >> fs[FOLDR_CONCR_EDGE]
+   >> rw[FOLDR_CONCR_EDGE]
+   >- fs[cE_equiv_def,MEM_EQUAL_def,MEM_SUBSET_def,COUNT_LIST_def]
+   >- (first_x_assum (qspec_then `λn. f (n + 1)` mp_tac)
+       >> `!i. i < LENGTH s ==> MEM (f (i + 1)) (EL i s)` by (
+            rpt strip_tac >> `MEM (f (SUC i)) (EL (SUC i) (h::s))` by fs[]
+            >> fs[EL,TL] >> metis_tac[DECIDE ``i+1=SUC i``]
+        )
+       >> simp[]
+       >> rpt strip_tac >> simp[d_conj_concr_def] >> rw[FOLDR_LEMM4]
+       >> fs[FOLDR_CONCR_EDGE]
+       >> qexists_tac `
+            concrEdge
+              (nub ((f 0).pos ++ x.pos))
+              (nub ((f 0).neg ++ x.neg))
+              (nub ((f 0).sucs ++ x.sucs))`
+       >> fs[] >> strip_tac
+       >- (fs[cE_equiv_def,MEM_EQUAL_SET] >> rpt strip_tac
+           >> Q.HO_MATCH_ABBREV_TAC `
+               set (g (f 0)) ∪
+               set
+               (FOLDR (λe pr. (g e) ⧺ pr) []
+                      (MAP (λn. f (n + 1)) (COUNT_LIST (LENGTH s)))) =
+               set (FOLDR (λe pr. (g e) ⧺ pr) []
+                          (MAP f (COUNT_LIST (SUC (LENGTH s)))))`
+           >> `MAP f (COUNT_LIST (SUC (LENGTH s)))
+               = f 0 :: MAP (λn. f (n + 1)) (COUNT_LIST (LENGTH s))` by (
+                simp[COUNT_LIST_def,MAP_MAP_o]
+                >> `(f o SUC) = (λn. f (n + 1))` suffices_by fs[]
+                >> `!n. (f o SUC) n = (λn. f (n + 1)) n` suffices_by metis_tac[]
+                >> fs[SUC_ONE_ADD]
+            )
+           >> rw[]
+          )
+       >- (qexists_tac `f 0` >> fs[]
+           >> qexists_tac `x` >> fs[FOLDR_CONCR_EDGE,concrEdge_component_equality]
+           >> `MEM (f 0) (EL 0 (h::s))`
+                by metis_tac[DECIDE ``0 < SUC (LENGTH s)``]
+           >> fs[EL,TL]
+          )
+      )
   );
-
 
 val GBA_TRANS_LEMM = store_thm
   ("GBA_TRANS_LEMM",
    ``!aP trns_concr_list.
-     ALL_DISTINCT (MAP SND trns_concr_list)
-   ∧ ALL_DISTINCT (MAP FST trns_concr_list)
-   (* ∧ (EVERY (ALL_DISTINCT o SND) trns_concr_list) *)
+      ALL_DISTINCT (MAP FST trns_concr_list)
    ==>
      let concr_edgs_list = MAP SND trns_concr_list
      in let to_abstr l = MAP (concr2AbstractEdge aP) l
-     in let abstr_trns_list = MAP to_abstr concr_edgs_list
-     in let abstr_trns_set = set (MAP set abstr_trns_list)
      in set (to_abstr (gba_trans_concr concr_edgs_list))
         = d_conj_set (set (MAP (λ(q,d). (q,set (to_abstr d)))
                                trns_concr_list)) (POW aP)``,
@@ -118,65 +246,86 @@ val GBA_TRANS_LEMM = store_thm
            >> fs[gba_trans_concr_def,concr2AbstractEdge_def,transformLabel_def]
           )
        >-(
-       `?f. y =
-          FOLDR
+       qabbrev_tac `s_ind =
+          GENLIST (λn. (EL n (MAP SND trns_concr_list),n))
+                  (LENGTH (MAP SND trns_concr_list))`
+       >> `?f. cE_equiv y
+          (FOLDR
               (λsF e.
                    <|pos := sF.pos ⧺ e.pos; neg := sF.neg ⧺ e.neg;
                      sucs := sF.sucs ⧺ e.sucs|>) (concrEdge [] [] [])
-              (MAP f (MAP SND trns_concr_list))
-              ∧ (!q. MEM q (MAP SND trns_concr_list)
-                     ==> MEM (f q) q)` by metis_tac[GBA_TRANS_LEMM1]
+              (MAP f s_ind))
+              ∧ (!q i. MEM (q,i) s_ind ==> MEM (f (q,i)) q)`
+           by metis_tac[GBA_TRANS_LEMM1]
        >> qabbrev_tac
             `a_sel = λq.
-              if ?d. MEM (q,d) trns_concr_list
-              then (let d = @x. MEM (q,x) trns_concr_list
+              if ?d i. (q,d) = EL i trns_concr_list
+                     ∧ i < LENGTH trns_concr_list
+              then (let d = @(x,i). (q,x) = EL i trns_concr_list
+                                  ∧ MEM (x,i) s_ind
                     in transformLabel aP (f d).pos (f d).neg)
               else ARB`
        >> qabbrev_tac
            `e_sel = λq.
-             if ?d. MEM (q,d) trns_concr_list
-             then (let d = @x. MEM (q,x) trns_concr_list
+             if ?d i. (q,d) = EL i trns_concr_list
+                    ∧ i < LENGTH trns_concr_list
+             then (let d = @(x,i). (q,x) = EL i trns_concr_list
+                                 ∧ MEM (x,i) s_ind
                    in set ((f d).sucs))
              else ARB`
-       >> `concr2AbstractEdge aP y =
+       >> qabbrev_tac `Y =
+                  (FOLDR
+                       (λsF e.
+                            <|pos := sF.pos ⧺ e.pos; neg := sF.neg ⧺ e.neg;
+                        sucs := sF.sucs ⧺ e.sucs|>) (concrEdge [] [] [])
+                       (MAP f s_ind))`
+       >> `concr2AbstractEdge aP Y ∈ d_conj_set s A`
+            suffices_by metis_tac[C2A_EDGE_CE_EQUIV]
+       >> `concr2AbstractEdge aP Y =
             ((POW aP) ∩ BIGINTER {a_sel q | q ∈ IMAGE FST s},
              BIGUNION {e_sel q | q ∈ IMAGE FST s})` by (
-            simp[concr2AbstractEdge_def,FOLDR_LEMM6]
+            qunabbrev_tac `Y`
+            >> simp[concr2AbstractEdge_def,FOLDR_LEMM6]
             >> rw[FOLDR_CONCR_EDGE] >> simp[concr2AbstractEdge_def]
             >> rpt strip_tac
             >- (simp[SET_EQ_SUBSET,SUBSET_DEF] >> rpt strip_tac
              >- (qunabbrev_tac `A` >> metis_tac[TRANSFORMLABEL_AP,SUBSET_DEF])
              >- (`x ∈ a_sel q` suffices_by rw[]
                  >> qunabbrev_tac `s` >> qunabbrev_tac `a_sel` >> fs[]
-                 >> `∃d. MEM (FST x',d) trns_concr_list` by (
+                 >> `∃d i. (FST x',d) = EL i trns_concr_list
+                          ∧ i < LENGTH trns_concr_list` by (
                     fs[MEM_ZIP,MEM_EL]
                     >> qexists_tac `SND (EL n' trns_concr_list)`
                     >> qexists_tac `n'` >> fs[LENGTH_MAP,EL_MAP]
                     >> Cases_on `EL n' trns_concr_list` >> fs[]
                  )
                  >> `x ∈ transformLabel aP
-                       (f (@x. MEM (FST x',x) trns_concr_list)).pos
-                       (f (@x. MEM (FST x',x) trns_concr_list)).neg`
+                       (f (@(x,i). (FST x',x) = EL i trns_concr_list
+                                 ∧ MEM (x,i) s_ind)).pos
+                       (f (@(x,i). (FST x',x) = EL i trns_concr_list
+                                 ∧ MEM (x,i) s_ind)).neg`
                   suffices_by metis_tac[]
-               >> `d = (@x. MEM (FST x',x) trns_concr_list)` by (
-                    `(λk. (k = d)) ($@ (λx. MEM (FST x',x) trns_concr_list))`
-                      suffices_by fs[]
-                    >> Q.HO_MATCH_ABBREV_TAC `Q ($@ M)`
-                    >> HO_MATCH_MP_TAC SELECT_ELIM_THM >> qunabbrev_tac `Q`
-                    >> rpt strip_tac >> fs[] >> qunabbrev_tac `M`
-                    >- metis_tac[]
-                    >- metis_tac[ALL_DISTINCT_PAIRS_LEMM]
+               >> qabbrev_tac `D = (@(x,i). (FST x',x) = EL i trns_concr_list
+                                          ∧ MEM (x,i) s_ind)`
+               >> `(FST x',FST D) = EL (SND D) trns_concr_list
+                   ∧ MEM D s_ind` by (
+                   `(λk. (FST x',FST k) = EL (SND k) trns_concr_list
+                         ∧ MEM k s_ind) D` suffices_by fs[]
+                   >> qunabbrev_tac `D` >> Q.HO_MATCH_ABBREV_TAC `(J ($@ Q))`
+                   >> HO_MATCH_MP_TAC SELECT_ELIM_THM >> qunabbrev_tac `J`
+                   >> qunabbrev_tac `Q` >> fs[] >> rpt strip_tac
+                   >- (qunabbrev_tac `s_ind` >> simp[MEM_GENLIST,MEM_EL]
+                       >> qexists_tac `(d,i)` >> fs[EL_MAP] >> rw[]
+                       >> Cases_on `EL i trns_concr_list` >> fs[]
+                      )
+                   >- (Cases_on `x''` >> fs[])
+                   >- (Cases_on `x''` >> fs[])
                )
-               >> `x ∈ transformLabel aP (f d).pos (f d).neg` suffices_by fs[]
-               >> `MEM (FST x', d) trns_concr_list` by metis_tac[SELECT_THM]
-               >> `MEM d (MAP SND trns_concr_list)` by (
-                    simp[MEM_MAP] >> qexists_tac `(FST x',d)` >> fs[]
+               >> `MEM (f D) (MAP f s_ind)` by (
+                    simp[MEM_MAP] >> qexists_tac `D` >> fs[]
+                    >> qexists_tac `(FST x',D)` >> fs[]
                )
-               >> `MEM (f d) (MAP f (MAP SND trns_concr_list))` by (
-                   simp[MEM_MAP] >> qexists_tac `d` >> fs[]
-                   >> qexists_tac `(FST x',d)` >> fs[]
-               )
-               >> metis_tac[TRANSFORMLABEL_SUBSET,FOLDR_APPEND,SUBSET_DEF]
+               >> metis_tac[TRANSFORMLABEL_SUBSET,FOLDR_APPEND_LEMM,SUBSET_DEF]
                 )
              >- (`!q. MEM q (MAP FST trns_concr_list) ==> x ∈ a_sel q` by (
                    rpt strip_tac >> fs[MEM_MAP]
@@ -185,76 +334,154 @@ val GBA_TRANS_LEMM = store_thm
                    >> `Q` suffices_by fs[] >> qunabbrev_tac `Q`
                    >> qexists_tac `q` >> rw[]
                    >> qunabbrev_tac `s` >> simp[MEM_MAP]
+                   >> rename [`MEM k trns_concr_list`]
                    >> qexists_tac
-                        `(λ(q,d). (q,set (MAP (concr2AbstractEdge aP) d))) y`
-                   >> simp[] >> Cases_on `y` >> simp[] >> qexists_tac `(q,r)`
+                        `(λ(q,d). (q,set (MAP (concr2AbstractEdge aP) d))) k`
+                   >> simp[]
+                   >> Cases_on `k` >> simp[] >> qexists_tac `(q,r)`
                    >> simp[]
                 )
-                >> `(∀e. MEM e (MAP f (MAP SND trns_concr_list))
+                >> `(∀e. MEM e (MAP f s_ind)
                       ⇒ x ∈ transformLabel aP e.pos e.neg) ∧ x ∈ POW aP`
                    suffices_by metis_tac[TRANSFORMLABEL_FOLDR]
                 >> rpt strip_tac >> fs[MEM_MAP]
-                >> `x ∈ a_sel (FST y')` by metis_tac[]
+                >> qunabbrev_tac `s_ind` >> fs[MEM_GENLIST]
+                >> `MEM (EL n trns_concr_list) trns_concr_list`
+                        by metis_tac[EL_MEM]
+                >> `?q d. EL n trns_concr_list = (q,d)` by (
+                     Cases_on `EL n trns_concr_list` >> fs[]
+                )
+                >> `MEM (q,d) trns_concr_list ∧ FST (q,d) = q` by fs[]
+                >> `x ∈ a_sel q` by metis_tac[MEM_EL]
                 >> qunabbrev_tac `a_sel` >> fs[]
                 >> `x ∈
                      transformLabel aP
-                     (f (@x. MEM (FST y',x) trns_concr_list)).pos
-                     (f (@x. MEM (FST y',x) trns_concr_list)).neg` by (
-                    `∃d. MEM (FST y',d) trns_concr_list` suffices_by metis_tac[]
-                    >> qexists_tac `SND y'` >> fs[]
+                     (f (@(x,i). (q,x) = EL i trns_concr_list
+                               ∧ i < LENGTH trns_concr_list
+                               ∧ (x = EL i (MAP SND trns_concr_list)))).pos
+                     (f (@(x,i). (q,x) = EL i trns_concr_list
+                               ∧ i < LENGTH trns_concr_list
+                               ∧ x = EL i (MAP SND trns_concr_list))).neg` by (
+                  `∃d i. (q,d) = EL i trns_concr_list
+                       ∧ (i < LENGTH trns_concr_list)` suffices_by metis_tac[]
+                  >> qexists_tac `d` >> fs[] >> metis_tac[MEM_EL]
                 )
-                >> `(@x. MEM (FST y',x) trns_concr_list) = SND y'` by (
-                    `(λk. (k = SND y')) ($@ (λx. MEM (FST y',x) trns_concr_list))`
+                >> `(@(x,i). (q,x) = EL i trns_concr_list
+                            ∧ i < LENGTH trns_concr_list
+                            ∧ (x = EL i (MAP SND trns_concr_list))) = (d,n)` by (
+                    `(λj. (j = (d,n)))
+                       ($@ (λ(x,i). (q,x) = EL i trns_concr_list
+                                  ∧ i < LENGTH trns_concr_list
+                                  ∧ (x = EL i (MAP SND trns_concr_list))))`
                       suffices_by fs[]
                     >> Q.HO_MATCH_ABBREV_TAC `Q ($@ M)`
                     >> HO_MATCH_MP_TAC SELECT_ELIM_THM >> qunabbrev_tac `Q`
                     >> rpt strip_tac >> fs[] >> qunabbrev_tac `M`
-                    >- (qexists_tac `SND y'` >> fs[])
-                    >- (Cases_on `y'` >> fs[]
-                        >> metis_tac[ALL_DISTINCT_PAIRS_LEMM])
+                    >- (qexists_tac `(d,n)` >> fs[EL_MAP])
+                    >- (Cases_on `x'` >> fs[] >> `r = n` suffices_by fs[EL_MAP]
+                        >> `EL n (MAP FST trns_concr_list) = q` by fs[EL_MAP]
+                        >> `EL r (MAP FST trns_concr_list) =
+                             FST (EL r trns_concr_list)` by metis_tac[EL_MAP]
+                        >> rw[] >> Cases_on `EL r trns_concr_list`
+                        >> rw[]
+                        >> `EL r (MAP FST trns_concr_list) =
+                             EL n (MAP FST trns_concr_list)` by fs[]
+                        >> metis_tac[ALL_DISTINCT_EL_IMP,LENGTH_MAP]
+                       )
                 )
-                >> Cases_on `y'` >> rw[] >> fs[]
+                >> `EL n (MAP SND trns_concr_list) = d` by fs[EL_MAP]
+                >> rw[] >> metis_tac[]
                 )
                )
             >- (`BIGUNION {e_sel q | ?x. q = FST x ∧ x ∈ s} =
                  BIGUNION {set d.sucs | MEM d
-                                          (MAP f (MAP SND trns_concr_list))}`
+                                        (MAP f s_ind)}`
                  by (
-                  `!q r. MEM (q,r) trns_concr_list
-                      ==> ((?d. MEM (q,d) trns_concr_list)
-                         ∧ (r = @x. MEM (q,x) trns_concr_list))` by (
+                  `!q r i. (q,r) = EL i trns_concr_list
+                         ∧ i < LENGTH trns_concr_list
+                      ==> ((?d n. (q,d) = EL n trns_concr_list)
+                         ∧ ((r,i) =
+                              @(x,i). (q,x) = EL i trns_concr_list
+                                    ∧ MEM (x,i) s_ind)
+                         ∧ ?n. n < LENGTH s_ind ∧ (r,i) = EL n s_ind)` by (
                       rpt strip_tac
                       >- metis_tac[]
-                      >- (`(λk. (k = r)) ($@ (λx. MEM (q,x)
-                                                  trns_concr_list))`
-                         suffices_by fs[]
+                      >- (`(λk. (k = (r,i)))
+                              ($@ (λ(x,j). (q,x) = EL j trns_concr_list
+                                         ∧ ?n. (n < LENGTH s_ind)
+                                             ∧ (x,j) = EL n s_ind))`
+                            suffices_by fs[MEM_EL]
                          >> Q.HO_MATCH_ABBREV_TAC `Q ($@ M)`
                          >> HO_MATCH_MP_TAC SELECT_ELIM_THM >> qunabbrev_tac `Q`
                          >> rpt strip_tac >> fs[] >> qunabbrev_tac `M`
-                         >- metis_tac[]
-                         >- metis_tac[ALL_DISTINCT_PAIRS_LEMM]
+                         >- (qexists_tac `(r,i)` >> fs[]
+                             >> qunabbrev_tac `s_ind` >> qexists_tac `i`
+                             >> simp[LENGTH_GENLIST,EL_MAP]
+                             >> Cases_on `EL i trns_concr_list` >> fs[]
+                            )
+                         >- (Cases_on `x` >> fs[]
+                             >> `EL i (MAP FST trns_concr_list) =
+                                  FST (EL i trns_concr_list)` by metis_tac[EL_MAP]
+                             >> `MEM (q',r') s_ind` by metis_tac[MEM_EL]
+                             >> qunabbrev_tac `s_ind` >> fs[MEM_GENLIST]
+                             >> `EL r' (MAP FST trns_concr_list) =
+                                  FST (EL r' trns_concr_list)` by metis_tac[EL_MAP]
+                             >> `r' = i` suffices_by
+                                  (rw[] >> fs[] >> Cases_on `EL i trns_concr_list`
+                                   >> fs[])
+                             >> Cases_on `EL i trns_concr_list`
+                             >> Cases_on `EL r' trns_concr_list` >> rw[] >> fs[]
+                             >> metis_tac[ALL_DISTINCT_EL_IMP,LENGTH_MAP])
+                         )
+                      >- (qunabbrev_tac `s_ind` >> qexists_tac `i`
+                          >> simp[LENGTH_GENLIST,EL_MAP]
+                          >> Cases_on `EL i trns_concr_list` >> fs[]
                          )
                   )
                   >> qunabbrev_tac `e_sel` >> simp[MEM_MAP] >> qunabbrev_tac `s`
                   >> simp[MEM_MAP,SET_EQ_SUBSET,SUBSET_DEF] >> rpt strip_tac
-                  >- (Cases_on `y` >> fs[] >> rw[]
-                      >> qexists_tac `set (f r).sucs` >> fs[] >> strip_tac
-                      >- metis_tac[]
-                      >- (qexists_tac `f r` >> fs[] >> qexists_tac `r` >> fs[]
-                         >> qexists_tac `(q,r)` >> fs[])
+                  >- (rename [`MEM k trns_concr_list`] >> fs[MEM_EL]
+                             >> rename[`k = EL i trns_concr_list`]
+                             >> Cases_on `k` >> fs[] >> rw[]
+                             >> qexists_tac `set (f (r,i)).sucs` >> fs[]
+                             >> first_x_assum (qspec_then `q` mp_tac) >> simp[]
+                             >> strip_tac
+                             >> first_x_assum (qspec_then `r` mp_tac) >> simp[]
+                             >> strip_tac
+                             >> first_x_assum (qspec_then `i` mp_tac) >> simp[]
+                             >> strip_tac >> rpt strip_tac
+                             >- metis_tac[]
+                             >- (qexists_tac `f (r,i)` >> fs[] >> rpt strip_tac
+                                >- metis_tac[MEM_EL]
+                                >- metis_tac[MEM_EL]
+                                >- (qexists_tac `(r,i)` >> fs[]
+                                    >> qexists_tac `n''` >> fs[]
+                                   )
+                                )
                      )
-                  >- (Cases_on `y'` >> fs[]
-                      >> qexists_tac `set d.sucs` >> fs[]
-                      >> qexists_tac `q` >> fs[] >> rpt strip_tac >> rw[]
-                      >- metis_tac[]
-                      >- metis_tac[]
-                      >- metis_tac[]
-                      >- (qexists_tac `(q,set (MAP (concr2AbstractEdge aP)r))`
-                          >> fs[] >> qexists_tac `(q,r)` >> fs[]
+                  >- (qunabbrev_tac `s_ind` >> fs[MEM_GENLIST]
+                      >> `MEM (EL n trns_concr_list) trns_concr_list` by fs[EL_MEM]
+                      >> `?q r. EL n trns_concr_list = (q,r)` by (
+                             Cases_on `EL n trns_concr_list` >> fs[]
+                       )
+                      >> first_x_assum (qspec_then `q` mp_tac) >> simp[]
+                      >> strip_tac
+                      >> first_x_assum (qspec_then `r` mp_tac) >> simp[]
+                      >> strip_tac
+                      >> first_x_assum (qspec_then `n` mp_tac) >> simp[]
+                      >> rpt strip_tac
+                      >> qexists_tac `set (f (r,n)).sucs` >> fs[]
+                      >> fs[] >> rpt strip_tac >> rw[] >> fs[]
+                      >- fs[EL_MAP]
+                      >- (qexists_tac `q`>> fs[] >> rw[]
+                          >- metis_tac[]
+                          >- metis_tac[]
+                          >- (qexists_tac `(q,set (MAP (concr2AbstractEdge aP)r))`
+                              >> fs[] >> qexists_tac `(q,r)` >> fs[])
                          )
                      )
-                    )
-                 >> metis_tac[FOLDR_APPEND,LIST_TO_SET,UNION_EMPTY]
+               )
+                 >> metis_tac[FOLDR_APPEND_LEMM,LIST_TO_SET,UNION_EMPTY]
                )
         )
        >> `(∀q d. (q,d) ∈ s ⇒ (a_sel q,e_sel q) ∈ d
@@ -262,35 +489,59 @@ val GBA_TRANS_LEMM = store_thm
            ∧ BIGINTER {a_sel q | q ∈ IMAGE FST s} ⊆ A`
            suffices_by metis_tac[FINITE_LIST_TO_SET,D_CONJ_SET_LEMM3]
        >> `!q r. (q,r) ∈ s
-           ==> (?d. MEM (q,d) trns_concr_list
+           ==> (?d i. (q,d) = EL i trns_concr_list
                  ∧ (r = set (MAP (concr2AbstractEdge aP) d))
-                 ∧ ((@x. MEM (q,x) trns_concr_list) = d))` by (
+                 ∧ (i < LENGTH trns_concr_list)
+                 ∧ ((@(x,i). (q,x) = EL i trns_concr_list
+                           ∧ MEM (x,i) s_ind) = (d,i)))` by (
             rpt strip_tac >> qunabbrev_tac `s` >> fs[MEM_MAP]
-            >> Cases_on `y'` >> fs[]
-            >> `r' = (@x. MEM (q',x) trns_concr_list)` by (
-                `(λk. (k = r')) ($@ (λx. MEM (q',x)
-                                        trns_concr_list))`
+            >> Cases_on `y'` >> fs[MEM_EL]
+            >> `(r',n') =
+                 (@(x,i). (q',x) = EL i trns_concr_list
+               ∧ (MEM (x,i) s_ind))` by (
+                `(λk. (k = (r',n')))
+                    ($@ (λ(x,i). (q',x) = EL i trns_concr_list
+                               ∧ MEM (x,i) s_ind))`
                   suffices_by fs[]
                 >> Q.HO_MATCH_ABBREV_TAC `Q ($@ M)`
                 >> HO_MATCH_MP_TAC SELECT_ELIM_THM >> qunabbrev_tac `Q`
                 >> rpt strip_tac >> fs[] >> qunabbrev_tac `M`
-                >- metis_tac[]
-                >- metis_tac[ALL_DISTINCT_PAIRS_LEMM]
+                >- (qexists_tac `(r',n')` >> fs[]
+                    >> qunabbrev_tac `s_ind` >> simp[MEM_GENLIST,EL_MAP]
+                    >> Cases_on `EL n' trns_concr_list` >> fs[])
+                >- (Cases_on `x'` >> fs[]
+                    >> `n' = r''` suffices_by (
+                         Cases_on `EL n' trns_concr_list`
+                         >> Cases_on `EL r'' trns_concr_list` >> rw[] >> fs[]
+                     ) >> rw[]
+                    >> `EL n' (MAP FST trns_concr_list) =
+                         FST (EL n' trns_concr_list)` by metis_tac[EL_MAP]
+                    >> qunabbrev_tac `s_ind` >> fs[MEM_GENLIST]
+                    >> `EL r'' (MAP FST trns_concr_list) =
+                         FST (EL r'' trns_concr_list)` by metis_tac[EL_MAP]
+                    >> Cases_on `EL n' trns_concr_list`
+                    >> Cases_on `EL r'' trns_concr_list` >> rw[] >> fs[]
+                    >> metis_tac[ALL_DISTINCT_EL_IMP,LENGTH_MAP]
+                   )
             )
-            >> rw[]
+            >> qexists_tac `r'` >> qexists_tac `n'` >> fs[]
+            >> simp[MEM_EL] >> qunabbrev_tac `s_ind` >> simp[MEM_GENLIST,EL_MAP]
         )
        >> rpt strip_tac
        >- (qunabbrev_tac `a_sel` >> qunabbrev_tac `e_sel`
            >> first_x_assum (qspec_then `q` mp_tac) >> rpt strip_tac
            >> first_x_assum (qspec_then `d` mp_tac) >> simp[] >> strip_tac
-           >> simp[MEM_MAP] >> qabbrev_tac `D = @x. MEM (q,x) trns_concr_list`
-           >> qexists_tac `f D` >> fs[]
+           >> simp[MEM_MAP]
+           >> qabbrev_tac `D = (d',i)`
+           >> qexists_tac `f D`
            >> `(transformLabel aP (f D).pos (f D).neg, set (f D).sucs) =
-                  concr2AbstractEdge aP (f D) ∧ MEM (f D) D`
+                  concr2AbstractEdge aP (f D) ∧ MEM (f D) d'`
               suffices_by metis_tac[]
            >> Cases_on `f D` >> simp[concr2AbstractEdge_def]
-           >> `MEM D (MAP SND trns_concr_list)` suffices_by metis_tac[]
-           >> fs[MEM_MAP] >> qexists_tac `(q,D)` >> fs[]
+           >> `MEM (d',i) s_ind` suffices_by metis_tac[]
+           >> qunabbrev_tac `s_ind` >> simp[MEM_GENLIST]
+           >> simp[EL_MAP]
+           >> Cases_on `EL i trns_concr_list` >> fs[]
           )
        >- (HO_MATCH_MP_TAC IN_BIGINTER_SUBSET >> fs[]
            >> qexists_tac `q` >> fs[] >> qexists_tac `(q,d)` >> fs[]
@@ -317,117 +568,208 @@ val GBA_TRANS_LEMM = store_thm
        )
     >- (
      `?a e. x = (a,e)` by (Cases_on `x` >> fs[])
-     >> `∀q d. (q,d) ∈ s ⇒ ∃a' e'. (a',e') ∈ d ∧ a ⊆ a' ∧ e' ⊆ e`
-         by metis_tac[D_CONJ_SET_LEMM2,FINITE_LIST_TO_SET]
-     >> `?f_a f_e.
-          !q d. (q,d) ∈ s ==> ((f_a q d,f_e q d) ∈ d
-                            ∧ (a ⊆ f_a q d) ∧ (f_e q d ⊆ e))`
-          by metis_tac[SKOLEM_THM]
+     >> `∃f_a f_e.
+          ∀q d.
+          ((q,d) ∈ s ⇒
+                 (f_a q d,f_e q d) ∈ d ∧ a ⊆ f_a q d ∧ f_e q d ⊆ e)
+          ∧ ((POW aP) ∩ BIGINTER {f_a q d | (q,d) ∈ s} = a)
+          ∧ (BIGUNION {f_e q d | (q,d) ∈ s} = e)`
+        by metis_tac[D_CONJ_SET_LEMM2_STRONG,FINITE_LIST_TO_SET]
      >> qunabbrev_tac `s` >> fs[MEM_MAP]
-     >> `?f. !y q d.
-          ((q,d) = (λ(q,d). (q,set (MAP (concr2AbstractEdge aP) d))) y)
-          ∧ (MEM y trns_concr_list)
-          ==> (MEM (f y) (SND y)
-             ∧ (concr2AbstractEdge aP (f y) = (f_a q d,f_e q d)))` by (
+     >> qabbrev_tac `c2a = concr2AbstractEdge aP` >> fs[]
+     >> `?f. !q d d_c i.
+          ((q,d) = (λ(q,d). (q,set (MAP c2a d))) (q,d_c))
+          ∧ ((q,d_c) = EL i trns_concr_list
+             ∧ i < LENGTH trns_concr_list)
+          ==> (MEM (f i) d_c
+             ∧ (c2a (f i) = (f_a q d,f_e q d)))` by (
          qabbrev_tac `sel =
-           λy.
-            if MEM y trns_concr_list
+           λi.
+            if i < LENGTH trns_concr_list
             then
-             let (q,d) = (λ(q,d). (q,set (MAP (concr2AbstractEdge aP) d))) y
-             in @cE. MEM cE (SND y)
+             let (q,d_c) = EL i trns_concr_list
+             in let d =
+                      set (MAP (concr2AbstractEdge aP) d_c)
+             in @cE. MEM cE d_c
                    ∧ concr2AbstractEdge aP cE = (f_a q d,f_e q d)
             else ARB`
          >> qexists_tac `sel` >> fs[] >> rpt gen_tac >> strip_tac
-         >> `sel y =
-              (λ(q,d).
+         >> `sel i =
                 @cE.
-                  MEM cE (SND y)
-                  ∧ concr2AbstractEdge aP cE = (f_a q d,f_e q d))
-                  ((λ(q,d). (q,set (MAP (concr2AbstractEdge aP) d))) y)` by (
-             qunabbrev_tac `sel` >> fs[]
+                  MEM cE d_c
+                  ∧ concr2AbstractEdge aP cE =
+                     (f_a q (set (MAP c2a d_c)),
+                      f_e q (set (MAP c2a d_c)))` by (
+             qunabbrev_tac `sel` >> fs[] >> simp[]
+             >> Cases_on `EL i trns_concr_list` >> fs[]
          )
-         >> `?q1 ce_list. y = (q1,ce_list)` by (Cases_on `y` >> fs[])
          >> fs[]
          >> Q.HO_MATCH_ABBREV_TAC
-              `MEM ($@ P) ce_list
-             ∧ concr2AbstractEdge aP ($@ P) = (A,E)`
-         >> qabbrev_tac `Q =
-                 λc. MEM c ce_list
-                   ∧ concr2AbstractEdge aP c = (A,E)`
+              `MEM ($@ P) d_c ∧ c2a ($@ P) = (A,E)`
+         >> qabbrev_tac `Q = λc. MEM c d_c ∧ c2a c = (A,E)`
          >> `Q ($@ P)` suffices_by fs[] >> HO_MATCH_MP_TAC SELECT_ELIM_THM
          >> qunabbrev_tac `P` >> qunabbrev_tac `Q` >> fs[]
+         >> qabbrev_tac `d = set (MAP c2a d_c)` >> fs[]
          >> first_x_assum (qspec_then `q` mp_tac) >> rpt strip_tac
          >> first_x_assum (qspec_then `d` mp_tac) >> rpt strip_tac
          >> `(f_a q d,f_e q d) ∈ d ∧ a ⊆ f_a q d ∧ f_e q d ⊆ e` by (
            `∃y.
             (q,d) = (λ(q,d). (q,set (MAP (concr2AbstractEdge aP) d))) y
                   ∧ MEM y trns_concr_list` suffices_by fs[]
-           >> qexists_tac `y` >> rw[] >> fs[]
+           >> qexists_tac `(q,d_c)` >> rw[] >> fs[EL_MEM]
          )
+         >> qunabbrev_tac `d`
          >> rw[] >> fs[MEM_MAP] >> metis_tac[]
      )
-     >> GBA_TRANS_LEMM2
-)
-)
-
-
-)
-
-
-
-   gen_tac
-   >> Induct_on `trns_concr_list`
-   >> fs[d_conj_set_def,gba_trans_concr_def]
-   >- (rw[ITSET_THM,ZIP_def]
-       >> simp[concr2AbstractEdge_def,transformLabel_def]
-      )
-   >- (rpt strip_tac
-       >> Q.HO_MATCH_ABBREV_TAC `
-           set (MAP c2A (d_conj_concr (SND h) (R_L)))
-            = ITSET (d_conj o SND)
-                    (((FST h,set (MAP c2A (SND h)))) INSERT
-                    R_R) {(POW aP,{})}`
-       >> `set (MAP c2A (d_conj_concr (SND h) R_L)) =
-           (d_conj o SND) (FST h,set (MAP c2A (SND h)))
-              (ITSET (d_conj o SND) (R_R DELETE (FST h,set (MAP c2A (SND h))))
-                     {(POW aP,{})})` suffices_by (
-            Q.HO_MATCH_ABBREV_TAC `A = B ==> A = C`
-            >> `C = B` suffices_by fs[] >> qunabbrev_tac `B`
-            >> qunabbrev_tac `C`
-            >> `FINITE R_R` suffices_by metis_tac[D_CONJ_SET_RECURSES]
-            >> metis_tac[FINITE_LIST_TO_SET]
+     >> `!d_c i. d_c = EL i (MAP SND trns_concr_list)
+               ∧ i < LENGTH (MAP SND trns_concr_list)
+                          ==> MEM (f i) d_c` by (
+         simp[MEM_MAP,EL_MAP] >> rpt strip_tac
+         >> qabbrev_tac `d_c = SND (EL i trns_concr_list)`
+         >> `?q. MEM (q,d_c) trns_concr_list
+               ∧ EL i trns_concr_list = (q,d_c)` by (
+             `MEM (EL i trns_concr_list) trns_concr_list` by fs[EL_MEM]
+             >> Cases_on `EL i trns_concr_list` >> qunabbrev_tac `d_c`
+             >> fs[] >> metis_tac[]
+         )
+         >> first_x_assum (qspec_then `q` mp_tac) >> rpt strip_tac
+         >> first_x_assum (qspec_then `set (MAP c2a d_c)` mp_tac)
+         >> rpt strip_tac
+         >> first_x_assum (qspec_then `d_c` mp_tac) >> rw[]
+     )
+     >> IMP_RES_TAC GBA_TRANS_LEMM2
+     >> `c2a
+          (FOLDR
+          (λsF e.
+               <|pos := sF.pos ⧺ e.pos; neg := sF.neg ⧺ e.neg;
+           sucs := sF.sucs ⧺ e.sucs|>) (concrEdge [] [] [])
+          (MAP f (COUNT_LIST (LENGTH (MAP SND trns_concr_list))))) = (a,e)`
+         suffices_by metis_tac[C2A_EDGE_CE_EQUIV]
+     >> rw[FOLDR_CONCR_EDGE] >> qunabbrev_tac `c2a`
+     >> simp[concr2AbstractEdge_def]
+     >> `(POW aP ∩ BIGINTER
+         {f_a q d |
+          ∃y.
+           (q,d) =
+             (λ(q,d). (q,set (MAP (concr2AbstractEdge aP) d))) y
+                     ∧ MEM y trns_concr_list} = a)
+       ∧ (BIGUNION
+          {f_e q d |
+           ∃y.
+            (q,d) =
+           (λ(q,d). (q,set (MAP (concr2AbstractEdge aP) d))) y
+          ∧ MEM y trns_concr_list} = e)` by (
+       `∃q d y.
+        (q,d) = (λ(q,d). (q,set (MAP (concr2AbstractEdge aP) d))) y
+      ∧ MEM y trns_concr_list` suffices_by (rpt strip_tac >> fs[] >> metis_tac[])
+       >> `?q d. MEM (q,d) trns_concr_list` by (
+           Cases_on `trns_concr_list` >> rw[] >> Cases_on `h` >> metis_tac[])
+       >> qexists_tac `q` >> fs[]
+       >> qexists_tac `set (MAP (concr2AbstractEdge aP) d)` >> fs[]
+       >> qexists_tac `(q,d)` >> fs[]
+     )
+     >> strip_tac
+     >- (simp[SET_EQ_SUBSET,SUBSET_DEF] >> rpt strip_tac >> fs[]
+      >- (rw[]
+          >- (fs[transformLabel_def] >> metis_tac[FOLDR_INTER,SUBSET_DEF])
+          >- (`?d_c. y = (q,d_c)` by (Cases_on `y` >> fs[])
+              >> `?i. (q,d_c) = EL i trns_concr_list
+                    ∧ i < LENGTH trns_concr_list` by metis_tac[MEM_EL]
+              >> `MEM (f i) d_c
+                ∧ concr2AbstractEdge aP (f i) =
+                   (f_a q (set (MAP (concr2AbstractEdge aP) d_c)),
+                    f_e q (set (MAP (concr2AbstractEdge aP) d_c)))`
+               by metis_tac[]
+              >> `(MEM_SUBSET (f i).pos
+                    (FOLDR (λe pr. e.pos ⧺ pr)
+                      [] (MAP f (COUNT_LIST
+                                     (LENGTH (MAP SND trns_concr_list))))))
+                ∧ (MEM_SUBSET (f i).neg
+                    (FOLDR (λe pr. e.neg ⧺ pr)
+                      [] (MAP f (COUNT_LIST
+                                     (LENGTH (MAP SND trns_concr_list))))))`
+                suffices_by (
+                Cases_on `f i` >> fs[concr2AbstractEdge_def]
+                >> Cases_on `EL i trns_concr_list` >> fs[] >> rw[]
+                >> metis_tac[TRANSFORMLABEL_SUBSET,SUBSET_DEF]
+              )
+              >> `MEM (f i) (MAP f (COUNT_LIST (LENGTH trns_concr_list)))`
+                     suffices_by (simp[] >> metis_tac[FOLDR_APPEND_LEMM])
+              >> simp[MEM_MAP] >> qexists_tac `i` >> fs[]
+              >> metis_tac[MEM_COUNT_LIST]
+             )
+          )
+      >- (rw[] >> fs[IN_INTER,IN_BIGINTER]
+          >> HO_MATCH_MP_TAC TRANSFORMLABEL_FOLDR >> rpt strip_tac
+          >- (POP_ASSUM mp_tac >> simp[MEM_MAP] >> rpt strip_tac
+              >> `y < LENGTH trns_concr_list` by fs[MEM_COUNT_LIST]
+              >> `MEM (f y) (EL y (MAP SND trns_concr_list))` by metis_tac[]
+              >> qabbrev_tac `d_c = EL y (MAP SND trns_concr_list)`
+              >> `?q. (q,d_c) = EL y trns_concr_list` by (
+                   `MEM (EL y trns_concr_list) trns_concr_list` by fs[EL_MEM]
+                   >> qunabbrev_tac `d_c` >> fs[]
+                   >> Cases_on `EL y trns_concr_list` >> rw[] >> simp[EL_MAP]
+               )
+              >> rw[]
+              >> qabbrev_tac `d = set (MAP (concr2AbstractEdge aP) d_c)`
+              >> first_x_assum (qspec_then `f_a q d` mp_tac)
+              >> simp[] >> rpt strip_tac
+              >> `x ∈ f_a q d` by (
+                 `(∃q' d'.
+                      f_a q d = f_a q' d'
+                    ∧ ∃y.
+                      (q',d') = (λ(q,d).
+                                  (q,set (MAP (concr2AbstractEdge aP) d))) y
+                    ∧ MEM y trns_concr_list)` suffices_by metis_tac[]
+                 >> qexists_tac `q` >> qexists_tac `d` >> fs[]
+                 >> qexists_tac `(q,d_c)` >> fs[EL_MEM]
+               )
+              >> first_x_assum (qspec_then `q` mp_tac) >> rpt strip_tac
+              >> first_x_assum (qspec_then `d_c` mp_tac) >> simp[]
+              >> rpt strip_tac >> first_x_assum (qspec_then `y` mp_tac)
+              >> simp[]
+              >> Cases_on `f y` >> fs[concr2AbstractEdge_def]
+             )
+          >- fs[]
+         )
         )
-       >> simp[d_conj_concr_def,SET_EQ_SUBSET,SUBSET_DEF] >> rpt strip_tac
-       >- (fs[MEM_MAP,FOLDR_LEMM4] 
-
-)
-
-       >> `R_R DELETE (FST h,set (MAP c2A (SND h))) = R_R` by (
-            `~((FST h,set (MAP c2A (SND h))) ∈ R_R)`
-               suffices_by metis_tac[DELETE_NON_ELEMENT]
-            >> CCONTR_TAC >> qunabbrev_tac `R_R` >> fs[MEM_ZIP]
-            >> `FST h = FST (EL n trns_concr_list)` by metis_tac[EL_MAP]
-            >> fs[MAP_MAP_o]
-            >> `set (MAP c2A (SND h)) =
-                 (set o (λl. MAP c2A l) o SND) (EL n trns_concr_list)`
-               by metis_tac[EL_MAP]
-            >> fs[]
-            >> `EL n trns_concr_list = h` by (
-                Cases_on `EL n trns_concr_list` >> Cases_on `h` >> fs[] >> rw[]
-                >> 
-)
- 
-)
-
-)
-
-
-
-
-)
-
-
-
+     >- (rw[] >> Q.HO_MATCH_ABBREV_TAC `S1 = BIGUNION S2`
+         >> `S2 = {set x.sucs |
+                     MEM x (MAP f (COUNT_LIST (LENGTH trns_concr_list))) }`
+            suffices_by (
+            qunabbrev_tac `S1` >> qunabbrev_tac `S2` >> fs[] >> rw[]
+            >> metis_tac[LIST_TO_SET,FOLDR_APPEND_LEMM,UNION_EMPTY]
+          )
+         >> qunabbrev_tac `S2` >> fs[] >> simp[SET_EQ_SUBSET,SUBSET_DEF]
+         >> rpt strip_tac
+         >- (`?d_c. y = (q,d_c)` by (Cases_on `y` >> fs[])
+             >> `?i. i < LENGTH trns_concr_list
+                   ∧ EL i trns_concr_list = (q,d_c)` by metis_tac[MEM_EL]
+             >> `concr2AbstractEdge aP (f i) =
+                 (f_a q (set (MAP (concr2AbstractEdge aP) d_c)),
+                  f_e q (set (MAP (concr2AbstractEdge aP) d_c)))`
+                by metis_tac[]
+             >> Cases_on `f i` >> fs[concr2AbstractEdge_def]
+             >> qexists_tac `f i` >> rw[] >> simp[MEM_MAP]
+             >> qexists_tac `i` >> fs[] >> metis_tac[MEM_COUNT_LIST]
+            )
+         >- (fs[MEM_MAP]
+             >> `?j. j = EL y trns_concr_list` by metis_tac[MEM_EL,MEM_COUNT_LIST]
+             >> `?q d_c. j = (q,d_c)` by (Cases_on `j` >> fs[])
+             >> `y < LENGTH (trns_concr_list)` by fs[MEM_COUNT_LIST]
+             >> `concr2AbstractEdge aP (f y) =
+                (f_a q (set (MAP (concr2AbstractEdge aP) d_c)),
+                 f_e q (set (MAP (concr2AbstractEdge aP) d_c)))`
+                by metis_tac[]
+             >> qabbrev_tac `d = set (MAP (concr2AbstractEdge aP) d_c)`
+             >> qexists_tac `q` >> qexists_tac `d` >> fs[]
+             >> Cases_on `f y` >> fs[concr2AbstractEdge_def]
+             >> rw[] >> qexists_tac `(q,d_c)` >> fs[EL_MEM]
+            )
+        )
+    )
+   )
+  );
 
 val tlg_concr_def = Define`
   tlg_concr (t1,acc_t1) (t2,acc_t2) =
@@ -455,108 +797,47 @@ val addNodeToGBA_def = Define`
     then g
     else addNode (nodeLabelGBA qs) g`;
 
+val ADDNODE_GBA_NOTWF_LEMM = store_thm
+  ("ADDNODE_GBA_NOTWF_LEMM",
+   ``!g qs. { x | inGBA (addNodeToGBA g qs) x } =
+             { x | inGBA g x } ∪ {qs} ``,
+   simp[SET_EQ_SUBSET,SUBSET_DEF] >> rpt strip_tac
+   >> fs[addNodeToGBA_def] >> Cases_on `inGBA g qs`
+   >> fs[] >> fs[inGBA_def]
+   >- (fs[EXISTS_MEM,MEM_MAP] >> `?i. y = (i,n)` by (Cases_on `y` >> fs[])
+       >> `lookup i (addNode (nodeLabelGBA qs) g).nodeInfo = SOME n`
+            by metis_tac[MEM_toAList]
+       >> disj1_tac >> qexists_tac `n` >> fs[] >> qexists_tac `y` >> fs[]
+       >> `lookup i g.nodeInfo = SOME n` suffices_by metis_tac[MEM_toAList]
+       >> fs[addNode_def] >> 
+)
+)
+
+
+
 val addEdgeToGBA_def = Define`
   addEdgeToGBA g id eL suc =
     case findNode (λ(i,q). MEM_EQUAL q.frmls suc) g of
       | SOME (i,q) =>  addEdge id (eL,i) g
       | NONE => NONE`;
 
-val concr_extrTrans_def = Define`
-  concr_extrTrans g_AA aa_id =
-    case lookup aa_id g_AA.followers of
-      | NONE => NONE
-      | SOME aa_edges =>
-        let aa_edges_with_frmls =
-            CAT_OPTIONS
-                (MAP
-                 (λ(eL,id).
-                   case lookup id g_AA.nodeInfo of
-                     | NONE => NONE
-                     | SOME n => SOME (eL,n.frml))
-                 aa_edges
-                )
-        in let aa_edges_grpd =
-               GROUP_BY
-                   (λ(eL1,f1) (eL2,f2). eL1.edge_grp = eL2.edge_grp)
-                   aa_edges_with_frmls
-        in let concr_edges:(α concrEdge) list =
-               CAT_OPTIONS
-                (MAP
-                 (λgrp. case grp of
-                          | [] => NONE
-                          | ((eL,f)::xs) =>
-                            SOME
-                             (concrEdge eL.pos_lab eL.neg_lab (f::MAP SND xs))
-                 ) aa_edges_grpd)
-        in do node <- lookup aa_id g_AA.nodeInfo ;
-              true_edges <-
-                SOME (MAP
-                       (λeL. (concrEdge eL.pos_lab eL.neg_lab []))
-                       node.true_labels) ;
-              SOME (concr_edges ++ true_edges)
-           od`;
 
+val extractGBATrans_def = Define`
+  extractGBATrans aP g q =
+    do (id,n) <- findNode (λ(i,n). ((set n.frmls) = q)) g ;
+       fls <- lookup id g.followers ;
+       SOME (
+         CAT_OPTIONS
+             (MAP (λ(eL,i).
+                    do nL <- lookup i g.nodeInfo ;
+                       SOME (
+                        (transformLabel aP eL.pos_lab eL.neg_lab,
+                         set nL.frmls)
+                       )
+                    od
+                  ) fls
+             )
+       )
+     od `;
 
-(*TODO: prove termination*)
-val expandGBA_def = Define`
-   (expandGBA g_AA acc [] G = SOME G)
- ∧ (expandGBA g_AA acc (id::ids) G =
-    case lookup id G.nodeInfo of
-      | NONE => NONE
-      | SOME current_node =>
-       let aa_frml_ids =
-            CAT_OPTIONS
-              (MAP (λf. OPTION_MAP FST
-                          (findNode (λ(i,l). l.frml = f) g_AA)
-                   )
-                  current_node.frmls)
-       in let concr_edges =
-               CAT_OPTIONS
-                 (MAP (concr_extrTrans g_AA) aa_frml_ids)
-       in let trans_unopt = gba_trans_concr concr_edges
-       in let flws_with_acc_sets =
-               MAP (λcE.
-                     let acc_sets =
-                      CAT_OPTIONS
-                         (MAP (λ(f,f_trans).
-                               if acc_cond_concr cE f f_trans
-                               then (SOME f)
-                               else NONE
-                             ) acc
-                         )
-                     in (cE,acc_sets)
-                   ) trans_unopt
-       in let trans = ONLY_MINIMAL tlg_concr flws_with_acc_sets
-       in let new_sucs =
-                FILTER (λqs. ~inGBA G qs)
-                   (MAP (λ(cE,fs). cE.sucs) trans)
-       in let (new_ids, G1) =
-                FOLDR (λn (ids,g). ((g.next::ids),addNodeToGBA g n))
-                      ([],G) new_sucs
-       in do G2 <-
-              FOLDR
-                (λ(eL,suc) g_opt. do g <- g_opt ;
-                                     addEdgeToGBA g id eL suc
-                                  od)
-                (SOME G1)
-                (MAP (λ(cE,f). (edgeLabelGBA cE.pos cE.neg f,cE.sucs)) trans) ;
-             expandGBA g_AA acc (ids ++ new_ids) G2
-          od
-   )`;
-
-val expandGBA_init_def = Define`
-  expandGBA_init (concrAA g_AA initAA props) =
-    let initNodes = MAP (λi_list.
-                          let suc_nLabels = MAP (λn. lookup i g_AA.nodeInfo)
-                          in MAP (λl. l.frml) (CAT_OPTIONS suc_nLabels)
-                        ) initAA
-    in let G0 = FOLDR addNodeToGraph empty initNodes
-    in let initIds = MAP FST (toAList G0)
-    in let acc_sets = FILTER is_until (graphStates g_AA)
-    in let graph = expandGBA g_AA acc_sets initIds G0
-    in concrGBA graph initIds props`;
-
-
-
-
-
+val _ = export_theory();
